theories/iris/iris_wp_def.v
@@ -65,8 +65,8 @@ Definition gen_heap_wasm_store `{!wasmG Σ} (s: store_record) : iProp Σ :=
    (gen_heap_interp (gmap_of_list s.(s_globals))) ∗
    (gen_heap_interp (gmap_of_list (fmap mem_length s.(s_mems)))) ∗
    (gen_heap_interp (gmap_of_list (fmap tab_size s.(s_tables)))) ∗
-   (gen_heap_interp (gmap_of_list (fmap mem_max_opt s.(s_mems)))) ∗
-   (gen_heap_interp (gmap_of_list (fmap table_max_opt s.(s_tables)))))%I.
+   (@gen_heap_interp _ _ _ _ _ memlimit_hsG (gmap_of_list (fmap mem_max_opt s.(s_mems)))) ∗
+   (@gen_heap_interp _ _ _ _ _ tablimit_hsG (gmap_of_list (fmap table_max_opt s.(s_tables)))))%I.
 
 (* TODO: let this use the above gen_heap as well. Currently too much a hassle as this needs to update every file. *)
 Global Instance heapG_irisG `{!wasmG Σ} : irisGS wasm_lang Σ := {
@@ -80,8 +80,8 @@ Global Instance heapG_irisG `{!wasmG Σ} : irisGS wasm_lang Σ := {
       (ghost_map_auth frameGName 1 (<[ tt := Build_frame locs inst ]> ∅)) ∗ 
       (gen_heap_interp (gmap_of_list (fmap mem_length s.(s_mems)))) ∗
       (gen_heap_interp (gmap_of_list (fmap tab_size s.(s_tables)))) ∗
-      (gen_heap_interp (gmap_of_list (fmap mem_max_opt s.(s_mems)))) ∗
-      (gen_heap_interp (gmap_of_list (fmap table_max_opt s.(s_tables))))
+      (@gen_heap_interp _ _ _ _ _ memlimit_hsG (gmap_of_list (fmap mem_max_opt s.(s_mems)))) ∗
+      (@gen_heap_interp _ _ _ _ _ tablimit_hsG (gmap_of_list (fmap table_max_opt s.(s_tables))))
       
     )%I;
     num_laters_per_step _ := 0;
@@ -127,7 +127,7 @@ Notation "n ↦[wt][ i ] v" := (mapsto (L:=N*N) (V:=funcelem) (n, i) (DfracOwn 1
                            (at level 20, format "n ↦[wt][ i ] v") : bi_scope.
 Notation "n ↪[wtsize] m" := (mapsto (L:=N) (V:=nat) n (DfracDiscarded) m%V)
                               (at level 20, format "n ↪[wtsize] m") : bi_scope.
-Notation "n ↪[wtlimit] m" := (mapsto (L:=N) (V:=option N) n (DfracDiscarded) m%V)
+Notation "n ↪[wtlimit] m" := (mapsto (L:=N) (V:=option N) (hG:=tablimit_hsG) n (DfracDiscarded) m%V)
                               (at level 20, format "n ↪[wtlimit] m") : bi_scope.
 Notation "n ↦[wm]{ q } [ i ] v" := (mapsto (L:=N*N) (V:=byte) (n, i) q v%V)
                            (at level 20, q at level 5, format "n ↦[wm]{ q } [ i ] v") : bi_scope.
@@ -135,7 +135,7 @@ Notation "n ↦[wm][ i ] v" := (mapsto (L:=N*N) (V:=byte) (n, i) (DfracOwn 1) v%
                            (at level 20, format "n ↦[wm][ i ] v") : bi_scope.
 Notation "n ↦[wmlength] v" := (mapsto (L:=N) (V:=N) n (DfracOwn 1) v% V)
                            (at level 20, format "n ↦[wmlength] v") : bi_scope.
-Notation "n ↪[wmlimit] v" := (mapsto (L:=N) (V:=option N) n (DfracDiscarded) v% V)
+Notation "n ↪[wmlimit] v" := (mapsto (L:=N) (V:=option N) (hG:=memlimit_hsG) n (DfracDiscarded) v% V)
                            (at level 20, format "n ↪[wmlimit] v") : bi_scope.
 Notation "n ↦[wg]{ q } v" := (mapsto (L:=N) (V:=global) n q v%V)
                            (at level 20, q at level 5, format "n ↦[wg]{ q } v").
